examples/Stack_peter/stack_check_mli.v
@@ -1,0 +1,184 @@
+Set Implicit Arguments.
+
+Require Import gospelstdlib_verified.
+
+Require Coq.ZArith.BinInt TLC.LibLogic TLC.LibRelation TLC.LibInt TLC.LibListZ.
+
+Require Import CFML.SepBase CFML.SepLifted CFML.WPLib CFML.WPLifted CFML.WPRecord CFML.WPArray CFML.WPBuiltin.
+
+Require CFML.Stdlib.Array_ml CFML.Stdlib.List_ml CFML.Stdlib.Sys_ml.
+
+Require Import Coq.ZArith.BinIntDef CFML.Semantics CFML.WPHeader.
+
+Delimit Scope Z_scope with Z.
+
+Import Stdlib.
+
+Import Gospelstdlib.
+
+Import List.
+
+Parameter t : Type -> Type.
+
+Module Type Stack.
+
+Parameter Stack :
+  forall a : Type,  
+  forall {Ea : CFML.SepLifted.Enc a},
+  list a ->
+  loc -> CFML.SepBase.SepBasicSetup.SepSimplArgsCredits.hprop.
+
+Parameter create : CFML.Semantics.val.
+
+Parameter create_spec :
+  forall a : Type,
+  forall {Ea : CFML.SepLifted.Enc a},
+  CFML.SepLifted.Triple (
+    CFML.SepLifted.Trm_apps create (
+      Coq.Lists.List.cons (
+        @CFML.SepLifted.dyn_make CFML.Semantics.val _ Coq.Init.Datatypes.tt
+      ) Coq.Lists.List.nil
+    )
+  ) CFML.SepBase.SepBasicSetup.SepSimplArgsCredits.hempty (
+    fun _prog_q : loc =>
+    CFML.SepBase.SepBasicSetup.HS.repr (Stack (@nil a )) _prog_q
+  ).
+
+Parameter is_empty : CFML.Semantics.val.
+
+Parameter is_empty_spec :
+  forall a : Type,
+  forall {Ea : CFML.SepLifted.Enc a},
+  forall _prog_q : loc,
+  forall q : list a,
+  CFML.SepLifted.Triple (
+    CFML.SepLifted.Trm_apps is_empty (
+      Coq.Lists.List.cons (@CFML.SepLifted.dyn_make loc _ _prog_q) Coq.Lists.List.nil
+    )
+  ) (CFML.SepBase.SepBasicSetup.HS.repr (Stack q) _prog_q) (
+    fun _prog_b : bool =>
+    CFML.SepBase.SepBasicSetup.SepSimplArgsCredits.hstar (
+        hpure (_prog_b = isTrue (Coq.Init.Logic.eq q (@nil a)))
+      ) (
+        CFML.SepBase.SepBasicSetup.HS.repr (Stack q) _prog_q
+    )
+  ).
+
+Parameter push : CFML.Semantics.val.
+
+Parameter push_spec :
+  forall a : Type,
+  forall {Ea : CFML.SepLifted.Enc a},
+  forall _prog_p : loc,
+  forall p : list a,
+  forall x : a,
+  CFML.SepLifted.Triple (
+    CFML.SepLifted.Trm_apps push (
+      Coq.Lists.List.cons (@CFML.SepLifted.dyn_make loc _ _prog_p) (
+        Coq.Lists.List.cons (@CFML.SepLifted.dyn_make a _ x) Coq.Lists.List.nil
+      )
+    )
+  ) (CFML.SepBase.SepBasicSetup.HS.repr (Stack p) _prog_p) (
+    fun _ : Coq.Init.Datatypes.unit =>
+    CFML.SepBase.SepBasicSetup.HS.repr (Stack (cons x p)) _prog_p
+  ).
+
+Parameter pop : CFML.Semantics.val.
+
+Parameter pop_spec :
+  forall a : Type,
+  forall {Ea : CFML.SepLifted.Enc a},
+  forall _prog_p : loc,
+  forall p : list a,
+  Coq.Init.Logic.not (Coq.Init.Logic.eq p (@nil a)) ->
+  CFML.SepLifted.Triple (
+    CFML.SepLifted.Trm_apps pop (
+      Coq.Lists.List.cons (@CFML.SepLifted.dyn_make loc _ _prog_p) Coq.Lists.List.nil
+    )
+  ) (CFML.SepBase.SepBasicSetup.HS.repr (Stack p) _prog_p) (
+    fun r : a =>
+    CFML.SepBase.SepBasicSetup.SepSimplArgsCredits.hexists (
+      fun _p_ : list a =>
+      CFML.SepBase.SepBasicSetup.SepSimplArgsCredits.hstar (
+        CFML.SepBase.SepBasicSetup.SepSimplArgsCredits.hpure (
+          Coq.Init.Logic.eq p (cons r _p_)
+        )
+      ) (
+        CFML.SepBase.SepBasicSetup.HS.repr (Stack _p_) _prog_p
+      )
+    )
+    ).
+
+Parameter clear : CFML.Semantics.val.
+
+Parameter clear_spec :
+  forall a : Type,  
+  forall {Ea : CFML.SepLifted.Enc a},
+  forall _prog_p : loc,
+  forall p : list a,
+  CFML.SepLifted.Triple (
+    CFML.SepLifted.Trm_apps clear (
+      Coq.Lists.List.cons (@CFML.SepLifted.dyn_make loc _ _prog_p) Coq.Lists.List.nil
+    )
+  ) (CFML.SepBase.SepBasicSetup.HS.repr (Stack p) _prog_p) (
+    fun _ : Coq.Init.Datatypes.unit =>
+    CFML.SepBase.SepBasicSetup.HS.repr (Stack (@nil a )) _prog_p
+  ).
+
+Parameter concat : CFML.Semantics.val.
+
+Parameter concat_spec :
+  forall a : Type,
+  forall {Ea : CFML.SepLifted.Enc a},
+  forall _prog_q1 : loc,
+  forall _prog_q2 : loc,    
+  forall q1 : list a,
+  forall q2 : list a,
+  CFML.SepLifted.Triple (
+    CFML.SepLifted.Trm_apps concat (
+      Coq.Lists.List.cons (@CFML.SepLifted.dyn_make loc _ _prog_q1) (
+        Coq.Lists.List.cons (@CFML.SepLifted.dyn_make loc _ _prog_q2) Coq.Lists.List.nil
+      )
+    )
+  ) (
+    CFML.SepBase.SepBasicSetup.SepSimplArgsCredits.hstar (
+      CFML.SepBase.SepBasicSetup.HS.repr (Stack q1) _prog_q1
+    ) (CFML.SepBase.SepBasicSetup.HS.repr (Stack q2) _prog_q2)
+  ) (
+    fun _ : Coq.Init.Datatypes.unit =>
+    CFML.SepBase.SepBasicSetup.SepSimplArgsCredits.hstar (
+      CFML.SepBase.SepBasicSetup.HS.repr (Stack (q1 ++ q2)) _prog_q1
+    ) (
+      CFML.SepBase.SepBasicSetup.HS.repr (Stack (@nil a )) _prog_q2
+    )
+  ).
+
+Parameter rev_append : CFML.Semantics.val.
+
+Parameter rev_append_spec :
+  forall a : Type,
+  forall {Ea : CFML.SepLifted.Enc a},
+  forall _prog_p1 : loc,
+  forall _prog_p2 : loc,
+  forall p1 : list a,
+  forall p2 : list a,
+  CFML.SepLifted.Triple (
+    CFML.SepLifted.Trm_apps rev_append (
+      Coq.Lists.List.cons (@CFML.SepLifted.dyn_make loc _ _prog_p1) (
+        Coq.Lists.List.cons (@CFML.SepLifted.dyn_make loc _ _prog_p2) Coq.Lists.List.nil
+      )
+    )
+  ) (
+    CFML.SepBase.SepBasicSetup.SepSimplArgsCredits.hstar (
+      CFML.SepBase.SepBasicSetup.HS.repr (Stack p1) _prog_p1
+    ) (CFML.SepBase.SepBasicSetup.HS.repr (Stack p2) _prog_p2)
+  ) (
+    fun _ : Coq.Init.Datatypes.unit =>
+    CFML.SepBase.SepBasicSetup.SepSimplArgsCredits.hstar (
+      CFML.SepBase.SepBasicSetup.HS.repr (Stack (@nil a )) _prog_p1
+    ) (
+      CFML.SepBase.SepBasicSetup.HS.repr (Stack (rev p1 ++ p2)) _prog_p2
+    )
+    ).
+
+End Stack.
