examples/translations/Alias/alias_mli.v
@@ -1,0 +1,60 @@
+Set Implicit Arguments.
+
+Require Import gospelstdlib_verified.
+
+Require Coq.ZArith.BinInt TLC.LibLogic TLC.LibRelation TLC.LibInt TLC.LibListZ.
+
+Require Import CFML.SepBase CFML.SepLifted CFML.WPLib CFML.WPLifted CFML.WPRecord CFML.WPArray CFML.WPBuiltin.
+
+Require CFML.Stdlib.Array_ml CFML.Stdlib.List_ml CFML.Stdlib.Sys_ml.
+
+Require Import Coq.ZArith.BinIntDef CFML.Semantics CFML.WPHeader.
+
+Delimit Scope Z_scope with Z.
+
+Import Stdlib.
+
+Import Gospelstdlib.
+
+Parameter t : Type.
+
+Parameter __Enc_t : CFML.SepLifted.Enc t.
+
+Instance _Enc_t : CFML.SepLifted.Enc t := __Enc_t.
+
+Parameter _Alias :
+  t -> t -> CFML.SepBase.SepBasicSetup.SepSimplArgsCredits.hprop.
+
+Parameter _st_eq : CFML.Semantics.val.
+
+Parameter _st_eq_spec :
+  forall _prog_x : t,
+  forall x : t,
+  forall _prog_y : t,
+  forall y : t,
+  CFML.SepLifted.Triple (
+    CFML.SepLifted.Trm_apps _st_eq (
+      Coq.Lists.List.cons (@CFML.SepLifted.dyn_make t _ _prog_x) (
+        Coq.Lists.List.cons (@CFML.SepLifted.dyn_make t _ _prog_y) Coq.Lists.List.nil
+      )
+    )
+  ) (
+    CFML.SepBase.SepBasicSetup.SepSimplArgsCredits.hstar (
+      CFML.SepBase.SepBasicSetup.HS.repr (_Alias x) _prog_x
+    ) (CFML.SepBase.SepBasicSetup.HS.repr (_Alias y) _prog_y)
+  ) (
+    fun _prog_b : bool =>
+    CFML.SepBase.SepBasicSetup.SepSimplArgsCredits.hstar (
+      CFML.SepBase.SepBasicSetup.HS.repr (_Alias x) _prog_x
+    ) (
+      CFML.SepBase.SepBasicSetup.SepSimplArgsCredits.hstar (
+        CFML.SepBase.SepBasicSetup.HS.repr (_Alias y) _prog_y
+      ) (
+        CFML.SepBase.SepBasicSetup.HS.repr (Bool (Coq.Init.Logic.eq x y)) _prog_b
+      )
+    )
+  ).
+
+Parameter _ph_eq : CFML.Semantics.val.
+
+
