examples/translations/Axiom/axiom_mli.v
@@ -1,0 +1,51 @@
+Set Implicit Arguments.
+
+Require Import gospelstdlib_verified.
+
+Require Coq.ZArith.BinInt TLC.LibLogic TLC.LibRelation TLC.LibInt TLC.LibListZ.
+
+Require Import CFML.SepBase CFML.SepLifted CFML.WPLib CFML.WPLifted CFML.WPRecord CFML.WPArray CFML.WPBuiltin.
+
+Require CFML.Stdlib.Array_ml CFML.Stdlib.List_ml CFML.Stdlib.Sys_ml.
+
+Require Import Coq.ZArith.BinIntDef CFML.Semantics CFML.WPHeader.
+
+Delimit Scope Z_scope with Z.
+
+Axiom add_ge :
+  forall x : Z,
+  forall y : Z,
+  Coq.Init.Logic.and (ge (plus x y) y) (ge (plus x y) x).
+
+Parameter T :
+  Z -> loc -> CFML.SepBase.SepBasicSetup.SepSimplArgsCredits.hprop.
+
+Axiom t_0 :
+  CFML.SepBase.SepBasicSetup.SepSimplArgsCredits.himpl CFML.SepBase.SepBasicSetup.SepSimplArgsCredits.hempty (
+    CFML.SepBase.SepBasicSetup.SepSimplArgsCredits.hforall (
+      fun _prog_t : Z =>
+      CFML.SepBase.SepBasicSetup.SepSimplArgsCredits.hforall (
+        fun t : Z =>
+        CFML.SepBase.SepBasicSetup.SepSimplArgsCredits.hwand (
+          CFML.SepBase.SepBasicSetup.HS.repr (T t) _prog_t
+        ) (
+          CFML.SepBase.SepBasicSetup.SepSimplArgsCredits.hstar (
+            CFML.SepBase.SepBasicSetup.SepSimplArgsCredits.hpure (eq t (0)%Z)
+          ) (CFML.SepBase.SepBasicSetup.HS.repr (T t) _prog_t)
+        )
+      )
+    )
+  ).
+
+Axiom extensionality :
+  forall {a48 : Type},
+  forall {Ih_a48 : Inhab a48},
+  forall s1 : sequence a48,
+  forall s2 : sequence a48,
+  Coq.Init.Logic.iff (eq s1 s2) (
+    forall i : Z,
+    Coq.Init.Logic.and (le (0)%Z i) (lt i (length s1)) ->
+    eq (seq_get s1 i) (seq_get s2 i)
+  ).
+
+
