examples/translations/BitSet/bitSet_mli.v
@@ -1,0 +1,140 @@
+Set Implicit Arguments.
+
+Require Import gospelstdlib_verified.
+
+Require Coq.ZArith.BinInt TLC.LibLogic TLC.LibRelation TLC.LibInt TLC.LibListZ.
+
+Require Import CFML.SepBase CFML.SepLifted CFML.WPLib CFML.WPLifted CFML.WPRecord CFML.WPArray CFML.WPBuiltin.
+
+Require CFML.Stdlib.Array_ml CFML.Stdlib.List_ml CFML.Stdlib.Sys_ml.
+
+Require Import Coq.ZArith.BinIntDef CFML.Semantics CFML.WPHeader.
+
+Delimit Scope Z_scope with Z.
+
+Import Stdlib.
+
+Import Gospelstdlib.
+
+Import _Set.
+
+Definition valid  (n : Coq.Numbers.BinNums.Z) : Prop:=
+Coq.Init.Logic.and (ge n (0)%Z) (lt n Sys.word_size).
+
+Parameter t : Type.
+
+Parameter __Enc_t : CFML.SepLifted.Enc t.
+
+Instance _Enc_t : CFML.SepLifted.Enc t := __Enc_t.
+
+Parameter BitSet :
+  set int -> t -> CFML.SepBase.SepBasicSetup.SepSimplArgsCredits.hprop.
+
+Parameter _singleton : CFML.Semantics.val.
+
+Lemma _singleton_spec :
+  forall _prog_v : int,
+  forall v : int,
+  CFML.SepLifted.Triple (
+    CFML.SepLifted.Trm_apps _singleton (
+      Coq.Lists.List.cons (@CFML.SepLifted.dyn_make int _ _prog_v) Coq.Lists.List.nil
+    )
+  ) (
+    CFML.SepBase.SepBasicSetup.SepSimplArgsCredits.hstar (
+      CFML.SepBase.SepBasicSetup.HS.repr (Int v) _prog_v
+    ) (CFML.SepBase.SepBasicSetup.SepSimplArgsCredits.hpure (valid v))
+  ) (
+    fun _prog_s : t =>
+    CFML.SepBase.SepBasicSetup.SepSimplArgsCredits.hstar (
+      CFML.SepBase.SepBasicSetup.HS.repr (Int v) _prog_v
+    ) (CFML.SepBase.SepBasicSetup.HS.repr (BitSet (singleton v)) _prog_s)
+  ). Admitted.
+
+Parameter _add : CFML.Semantics.val.
+
+Lemma _add_spec :
+  forall _prog_i : int,
+  forall i : int,
+  forall _prog_s1 : t,
+  forall s1 : set int,
+  CFML.SepLifted.Triple (
+    CFML.SepLifted.Trm_apps _add (
+      Coq.Lists.List.cons (@CFML.SepLifted.dyn_make int _ _prog_i) (
+        Coq.Lists.List.cons (@CFML.SepLifted.dyn_make t _ _prog_s1) Coq.Lists.List.nil
+      )
+    )
+  ) (
+    CFML.SepBase.SepBasicSetup.SepSimplArgsCredits.hstar (
+      CFML.SepBase.SepBasicSetup.HS.repr (Int i) _prog_i
+    ) (
+      CFML.SepBase.SepBasicSetup.SepSimplArgsCredits.hstar (
+        CFML.SepBase.SepBasicSetup.HS.repr (BitSet s1) _prog_s1
+      ) (CFML.SepBase.SepBasicSetup.SepSimplArgsCredits.hpure (valid i))
+    )
+  ) (
+    fun _prog_s2 : t =>
+    CFML.SepBase.SepBasicSetup.SepSimplArgsCredits.hstar (
+      CFML.SepBase.SepBasicSetup.HS.repr (Int i) _prog_i
+    ) (
+      CFML.SepBase.SepBasicSetup.SepSimplArgsCredits.hstar (
+        CFML.SepBase.SepBasicSetup.HS.repr (BitSet s1) _prog_s1
+      ) (CFML.SepBase.SepBasicSetup.HS.repr (BitSet (add i s1)) _prog_s2)
+    )
+  ). Admitted.
+
+Parameter _remove : CFML.Semantics.val.
+
+Lemma _remove_spec :
+  forall _prog_i : int,
+  forall i : int,
+  forall _prog_s1 : t,
+  forall s1 : set int,
+  CFML.SepLifted.Triple (
+    CFML.SepLifted.Trm_apps _remove (
+      Coq.Lists.List.cons (@CFML.SepLifted.dyn_make int _ _prog_i) (
+        Coq.Lists.List.cons (@CFML.SepLifted.dyn_make t _ _prog_s1) Coq.Lists.List.nil
+      )
+    )
+  ) (
+    CFML.SepBase.SepBasicSetup.SepSimplArgsCredits.hstar (
+      CFML.SepBase.SepBasicSetup.HS.repr (Int i) _prog_i
+    ) (
+      CFML.SepBase.SepBasicSetup.SepSimplArgsCredits.hstar (
+        CFML.SepBase.SepBasicSetup.HS.repr (BitSet s1) _prog_s1
+      ) (CFML.SepBase.SepBasicSetup.SepSimplArgsCredits.hpure (valid i))
+    )
+  ) (
+    fun _prog_s2 : t =>
+    CFML.SepBase.SepBasicSetup.SepSimplArgsCredits.hstar (
+      CFML.SepBase.SepBasicSetup.HS.repr (Int i) _prog_i
+    ) (
+      CFML.SepBase.SepBasicSetup.SepSimplArgsCredits.hstar (
+        CFML.SepBase.SepBasicSetup.HS.repr (BitSet s1) _prog_s1
+      ) (CFML.SepBase.SepBasicSetup.HS.repr (BitSet (remove i s1)) _prog_s2)
+    )
+  ). Admitted.
+
+Parameter _is_singleton : CFML.Semantics.val.
+
+Lemma _is_singleton_spec :
+  forall _prog_s : t,
+  forall s : set int,
+  CFML.SepLifted.Triple (
+    CFML.SepLifted.Trm_apps _is_singleton (
+      Coq.Lists.List.cons (@CFML.SepLifted.dyn_make t _ _prog_s) Coq.Lists.List.nil
+    )
+  ) (CFML.SepBase.SepBasicSetup.HS.repr (BitSet s) _prog_s) (
+    fun _prog_b : bool =>
+    CFML.SepBase.SepBasicSetup.SepSimplArgsCredits.hstar (
+      CFML.SepBase.SepBasicSetup.HS.repr (BitSet s) _prog_s
+    ) (
+      CFML.SepBase.SepBasicSetup.HS.repr (
+        Bool (
+          Coq.Init.Logic.ex (
+            fun v : int =>
+            Coq.Init.Logic.eq s (_Set.singleton v)
+          )
+        )
+      ) _prog_b
+    )
+  ). Admitted.
