examples/translations/Dyn_array/dyn_array_mli.v
@@ -1,0 +1,414 @@
+Set Implicit Arguments.
+
+Require Import gospelstdlib_verified.
+
+Require Coq.ZArith.BinInt TLC.LibLogic TLC.LibRelation TLC.LibInt TLC.LibListZ.
+
+Require Import CFML.SepBase CFML.SepLifted CFML.WPLib CFML.WPLifted CFML.WPRecord CFML.WPArray CFML.WPBuiltin.
+
+Require CFML.Stdlib.Array_ml CFML.Stdlib.List_ml CFML.Stdlib.Sys_ml.
+
+Require Import Coq.ZArith.BinIntDef CFML.Semantics CFML.WPHeader.
+
+Delimit Scope Z_scope with Z.
+
+Import Stdlib.
+
+Import Gospelstdlib.
+
+Import Sequence.
+
+Parameter t : Type.
+
+Parameter __Enc_t : CFML.SepLifted.Enc t.
+
+Instance _Enc_t : CFML.SepLifted.Enc t := __Enc_t.
+
+Parameter Dyn_array :
+  sequence int ->
+  loc -> CFML.SepBase.SepBasicSetup.SepSimplArgsCredits.hprop.
+
+Parameter _create : CFML.Semantics.val.
+
+Lemma _create_spec :
+  CFML.SepLifted.Triple (
+    CFML.SepLifted.Trm_apps _create (
+      Coq.Lists.List.cons (
+        @CFML.SepLifted.dyn_make CFML.Semantics.val _ Coq.Init.Datatypes.tt
+      ) Coq.Lists.List.nil
+    )
+  ) CFML.SepBase.SepBasicSetup.SepSimplArgsCredits.hempty (
+    fun _prog_a : loc =>
+    CFML.SepBase.SepBasicSetup.HS.repr (Dyn_array empty) _prog_a
+  ). Admitted.
+
+Parameter _make : CFML.Semantics.val.
+
+Lemma _make_spec :
+  forall _prog_n : int,
+  forall n : int,
+  forall _prog_e : int,
+  forall e : int,
+  CFML.SepLifted.Triple (
+    CFML.SepLifted.Trm_apps _make (
+      Coq.Lists.List.cons (@CFML.SepLifted.dyn_make int _ _prog_n) (
+        Coq.Lists.List.cons (@CFML.SepLifted.dyn_make int _ _prog_e) Coq.Lists.List.nil
+      )
+    )
+  ) (
+    CFML.SepBase.SepBasicSetup.SepSimplArgsCredits.hstar (
+      CFML.SepBase.SepBasicSetup.HS.repr (Int n) _prog_n
+    ) (CFML.SepBase.SepBasicSetup.HS.repr (Int e) _prog_e)
+  ) (
+    fun _prog_a : loc =>
+    CFML.SepBase.SepBasicSetup.SepSimplArgsCredits.hstar (
+      CFML.SepBase.SepBasicSetup.HS.repr (Int n) _prog_n
+    ) (
+      CFML.SepBase.SepBasicSetup.SepSimplArgsCredits.hstar (
+        CFML.SepBase.SepBasicSetup.HS.repr (Int e) _prog_e
+      ) (
+        CFML.SepBase.SepBasicSetup.HS.repr (
+          Dyn_array (init n (fun _ : Coq.Numbers.BinNums.Z => e))
+        ) _prog_a
+      )
+    )
+  ). Admitted.
+
+Parameter _get : CFML.Semantics.val.
+
+Lemma _get_spec :
+  forall _prog_a : loc,
+  forall a : sequence int,
+  forall _prog_i : int,
+  forall i : int,
+  CFML.SepLifted.Triple (
+    CFML.SepLifted.Trm_apps _get (
+      Coq.Lists.List.cons (@CFML.SepLifted.dyn_make loc _ _prog_a) (
+        Coq.Lists.List.cons (@CFML.SepLifted.dyn_make int _ _prog_i) Coq.Lists.List.nil
+      )
+    )
+  ) (
+    CFML.SepBase.SepBasicSetup.SepSimplArgsCredits.hstar (
+      CFML.SepBase.SepBasicSetup.HS.repr (Dyn_array a) _prog_a
+    ) (CFML.SepBase.SepBasicSetup.HS.repr (Int i) _prog_i)
+  ) (
+    fun _prog_r : int =>
+    CFML.SepBase.SepBasicSetup.SepSimplArgsCredits.hstar (
+      CFML.SepBase.SepBasicSetup.HS.repr (Dyn_array a) _prog_a
+    ) (
+      CFML.SepBase.SepBasicSetup.SepSimplArgsCredits.hstar (
+        CFML.SepBase.SepBasicSetup.HS.repr (Int i) _prog_i
+      ) (CFML.SepBase.SepBasicSetup.HS.repr (Int (seq_get a i)) _prog_r)
+    )
+  ). Admitted.
+
+Parameter _set : CFML.Semantics.val.
+
+Parameter _set_spec :
+  forall _prog_a : loc,
+  forall a : sequence int,
+  forall _prog_i : int,
+  forall i : int,
+  forall _prog_e : int,
+  forall e : int,
+  CFML.SepLifted.Triple (
+    CFML.SepLifted.Trm_apps _set (
+      Coq.Lists.List.cons (@CFML.SepLifted.dyn_make loc _ _prog_a) (
+        Coq.Lists.List.cons (@CFML.SepLifted.dyn_make int _ _prog_i) (
+          Coq.Lists.List.cons (@CFML.SepLifted.dyn_make int _ _prog_e) Coq.Lists.List.nil
+        )
+      )
+    )
+  ) (
+    CFML.SepBase.SepBasicSetup.SepSimplArgsCredits.hstar (
+      CFML.SepBase.SepBasicSetup.HS.repr (Dyn_array a) _prog_a
+    ) (
+      CFML.SepBase.SepBasicSetup.SepSimplArgsCredits.hstar (
+        CFML.SepBase.SepBasicSetup.HS.repr (Int i) _prog_i
+      ) (
+        CFML.SepBase.SepBasicSetup.SepSimplArgsCredits.hstar (
+          CFML.SepBase.SepBasicSetup.HS.repr (Int e) _prog_e
+        ) (
+          CFML.SepBase.SepBasicSetup.SepSimplArgsCredits.hpure (
+            Coq.Init.Logic.and (le (0)%Z i) (lt i (length a))
+          )
+        )
+      )
+    )
+  ) (
+    fun _ : Coq.Init.Datatypes.unit =>
+    CFML.SepBase.SepBasicSetup.SepSimplArgsCredits.hstar (
+      CFML.SepBase.SepBasicSetup.HS.repr (Dyn_array (set a i e)) _prog_a
+    ) (
+      CFML.SepBase.SepBasicSetup.SepSimplArgsCredits.hstar (
+        CFML.SepBase.SepBasicSetup.HS.repr (Int i) _prog_i
+      ) (CFML.SepBase.SepBasicSetup.HS.repr (Int e) _prog_e)
+    )
+  ).
+
+Parameter _length : CFML.Semantics.val.
+
+Parameter _length_spec :
+  forall _prog_a : loc,
+  forall a : sequence int,
+  CFML.SepLifted.Triple (
+    CFML.SepLifted.Trm_apps _length (
+      Coq.Lists.List.cons (@CFML.SepLifted.dyn_make loc _ _prog_a) Coq.Lists.List.nil
+    )
+  ) (CFML.SepBase.SepBasicSetup.HS.repr (Dyn_array a) _prog_a) (
+    fun _prog_l : int =>
+    CFML.SepBase.SepBasicSetup.SepSimplArgsCredits.hexists (
+      fun l : int =>
+      CFML.SepBase.SepBasicSetup.SepSimplArgsCredits.hstar (
+        CFML.SepBase.SepBasicSetup.HS.repr (Dyn_array a) _prog_a
+      ) (
+        CFML.SepBase.SepBasicSetup.SepSimplArgsCredits.hstar (
+          CFML.SepBase.SepBasicSetup.HS.repr (Int l) _prog_l
+        ) (
+          CFML.SepBase.SepBasicSetup.SepSimplArgsCredits.hpure (
+            Coq.Init.Logic.eq l (length a)
+          )
+        )
+      )
+    )
+  ).
+
+Parameter _is_empty : CFML.Semantics.val.
+
+Parameter _is_empty_spec :
+  forall _prog_a : loc,
+  forall a : sequence int,
+  CFML.SepLifted.Triple (
+    CFML.SepLifted.Trm_apps _is_empty (
+      Coq.Lists.List.cons (@CFML.SepLifted.dyn_make loc _ _prog_a) Coq.Lists.List.nil
+    )
+  ) (CFML.SepBase.SepBasicSetup.HS.repr (Dyn_array a) _prog_a) (
+    fun _prog_b : bool =>
+    CFML.SepBase.SepBasicSetup.SepSimplArgsCredits.hstar (
+      CFML.SepBase.SepBasicSetup.HS.repr (Dyn_array a) _prog_a
+    ) (
+      CFML.SepBase.SepBasicSetup.HS.repr (Bool (Coq.Init.Logic.eq a empty)) _prog_b
+    )
+  ).
+
+Parameter _find_last : CFML.Semantics.val.
+
+Parameter _find_last_spec :
+  forall _prog_a : loc,
+  forall a : sequence int,
+  CFML.SepLifted.Triple (
+    CFML.SepLifted.Trm_apps _find_last (
+      Coq.Lists.List.cons (@CFML.SepLifted.dyn_make loc _ _prog_a) Coq.Lists.List.nil
+    )
+  ) (CFML.SepBase.SepBasicSetup.HS.repr (Dyn_array a) _prog_a) (
+    fun _prog_r : option int =>
+    CFML.SepBase.SepBasicSetup.SepSimplArgsCredits.hexists (
+      fun r : option int =>
+      CFML.SepBase.SepBasicSetup.SepSimplArgsCredits.hstar (
+        CFML.SepBase.SepBasicSetup.HS.repr (Dyn_array a) _prog_a
+      ) (
+        CFML.SepBase.SepBasicSetup.SepSimplArgsCredits.hstar (
+          CFML.SepBase.SepBasicSetup.HS.repr (Option r) _prog_r
+        ) (
+          CFML.SepBase.SepBasicSetup.SepSimplArgsCredits.hpure (
+            match r with
+            | None => Coq.Init.Logic.and (Coq.Init.Logic.eq a empty) (
+                Coq.Init.Logic.eq a empty
+              )
+              | Some r => Coq.Init.Logic.eq r (
+                seq_get a (minus (length a) (1)%Z)
+              )
+              end
+          )
+        )
+      )
+    )
+  ).
+
+Parameter _copy : CFML.Semantics.val.
+
+Parameter _copy_spec :
+  forall _prog_a : loc,
+  forall a : sequence int,
+  CFML.SepLifted.Triple (
+    CFML.SepLifted.Trm_apps _copy (
+      Coq.Lists.List.cons (@CFML.SepLifted.dyn_make loc _ _prog_a) Coq.Lists.List.nil
+    )
+  ) (CFML.SepBase.SepBasicSetup.HS.repr (Dyn_array a) _prog_a) (
+    fun _prog_c : loc =>
+    CFML.SepBase.SepBasicSetup.SepSimplArgsCredits.hstar (
+      CFML.SepBase.SepBasicSetup.HS.repr (Dyn_array a) _prog_a
+    ) (CFML.SepBase.SepBasicSetup.HS.repr (Dyn_array a) _prog_c)
+  ).
+
+Parameter _add_last : CFML.Semantics.val.
+
+Parameter _add_last_spec :
+  forall _prog_a : loc,
+  forall a : sequence int,
+  forall _prog_e : int,
+  forall e : int,
+  CFML.SepLifted.Triple (
+    CFML.SepLifted.Trm_apps _add_last (
+      Coq.Lists.List.cons (@CFML.SepLifted.dyn_make loc _ _prog_a) (
+        Coq.Lists.List.cons (@CFML.SepLifted.dyn_make int _ _prog_e) Coq.Lists.List.nil
+      )
+    )
+  ) (
+    CFML.SepBase.SepBasicSetup.SepSimplArgsCredits.hstar (
+      CFML.SepBase.SepBasicSetup.HS.repr (Dyn_array a) _prog_a
+    ) (CFML.SepBase.SepBasicSetup.HS.repr (Int e) _prog_e)
+  ) (
+    fun _ : Coq.Init.Datatypes.unit =>
+    CFML.SepBase.SepBasicSetup.SepSimplArgsCredits.hstar (
+      CFML.SepBase.SepBasicSetup.HS.repr (Dyn_array (app a (singleton e))) _prog_a
+    ) (CFML.SepBase.SepBasicSetup.HS.repr (Int e) _prog_e)
+  ).
+
+Parameter _append : CFML.Semantics.val.
+
+Parameter _append_spec :
+  forall _prog_a1 : loc,
+  forall a1 : sequence int,
+  forall _prog_a2 : loc,
+  forall a2 : sequence int,
+  CFML.SepLifted.Triple (
+    CFML.SepLifted.Trm_apps _append (
+      Coq.Lists.List.cons (@CFML.SepLifted.dyn_make loc _ _prog_a1) (
+        Coq.Lists.List.cons (@CFML.SepLifted.dyn_make loc _ _prog_a2) Coq.Lists.List.nil
+      )
+    )
+  ) (
+    CFML.SepBase.SepBasicSetup.SepSimplArgsCredits.hstar (
+      CFML.SepBase.SepBasicSetup.HS.repr (Dyn_array a1) _prog_a1
+    ) (CFML.SepBase.SepBasicSetup.HS.repr (Dyn_array a2) _prog_a2)
+  ) (
+    fun _ : Coq.Init.Datatypes.unit =>
+    CFML.SepBase.SepBasicSetup.SepSimplArgsCredits.hstar (
+      CFML.SepBase.SepBasicSetup.HS.repr (Dyn_array (app a1 a2)) _prog_a1
+    ) (CFML.SepBase.SepBasicSetup.HS.repr (Dyn_array a2) _prog_a2)
+  ).
+
+Parameter _pop_last_opt : CFML.Semantics.val.
+
+Parameter _pop_last_opt_spec :
+  forall _prog_a : loc,
+  forall a : sequence int,
+  CFML.SepLifted.Triple (
+    CFML.SepLifted.Trm_apps _pop_last_opt (
+      Coq.Lists.List.cons (@CFML.SepLifted.dyn_make loc _ _prog_a) Coq.Lists.List.nil
+    )
+  ) (CFML.SepBase.SepBasicSetup.HS.repr (Dyn_array a) _prog_a) (
+    fun _prog_r : option int =>
+    CFML.SepBase.SepBasicSetup.SepSimplArgsCredits.hexists (
+      fun _a_ : sequence int =>
+      CFML.SepBase.SepBasicSetup.SepSimplArgsCredits.hexists (
+        fun r : option int =>
+        CFML.SepBase.SepBasicSetup.SepSimplArgsCredits.hstar (
+          CFML.SepBase.SepBasicSetup.HS.repr (Dyn_array _a_) _prog_a
+        ) (
+          CFML.SepBase.SepBasicSetup.SepSimplArgsCredits.hstar (
+            CFML.SepBase.SepBasicSetup.HS.repr (Option r) _prog_r
+          ) (
+            CFML.SepBase.SepBasicSetup.SepSimplArgsCredits.hpure (
+              match r with
+              | None => Coq.Init.Logic.and (Coq.Init.Logic.eq _a_ empty) (
+                  Coq.Init.Logic.eq a empty
+                )
+                | Some r => Coq.Init.Logic.eq (app _a_ (singleton r)) a
+                end
+            )
+          )
+        )
+      )
+    )
+  ).
+
+Parameter _remove_last : CFML.Semantics.val.
+
+Parameter _remove_last_spec :
+  forall _prog_a : loc,
+  forall a : sequence int,
+  CFML.SepLifted.Triple (
+    CFML.SepLifted.Trm_apps _remove_last (
+      Coq.Lists.List.cons (@CFML.SepLifted.dyn_make loc _ _prog_a) Coq.Lists.List.nil
+    )
+  ) (CFML.SepBase.SepBasicSetup.HS.repr (Dyn_array a) _prog_a) (
+    fun _ : Coq.Init.Datatypes.unit =>
+    CFML.SepBase.SepBasicSetup.SepSimplArgsCredits.hexists (
+      fun _a_ : sequence int =>
+      CFML.SepBase.SepBasicSetup.SepSimplArgsCredits.hstar (
+        CFML.SepBase.SepBasicSetup.HS.repr (Dyn_array _a_) _prog_a
+      ) (
+        CFML.SepBase.SepBasicSetup.SepSimplArgsCredits.hstar (
+          CFML.SepBase.SepBasicSetup.SepSimplArgsCredits.hpure (
+            Coq.Init.Logic.eq a empty -> Coq.Init.Logic.eq _a_ empty
+          )
+        ) (
+          CFML.SepBase.SepBasicSetup.SepSimplArgsCredits.hpure (
+            Coq.Init.Logic.not (Coq.Init.Logic.eq _a_ empty) ->
+            Coq.Init.Logic.eq _a_ (seq_sub_r a (minus (length a) (1)%Z))
+          )
+        )
+      )
+    )
+  ).
+
+Parameter _truncate : CFML.Semantics.val.
+
+Parameter _truncate_spec :
+  forall _prog_a : loc,
+  forall a : sequence int,
+  forall _prog_n : int,
+  forall n : int,
+  CFML.SepLifted.Triple (
+    CFML.SepLifted.Trm_apps _truncate (
+      Coq.Lists.List.cons (@CFML.SepLifted.dyn_make loc _ _prog_a) (
+        Coq.Lists.List.cons (@CFML.SepLifted.dyn_make int _ _prog_n) Coq.Lists.List.nil
+      )
+    )
+  ) (
+    CFML.SepBase.SepBasicSetup.SepSimplArgsCredits.hstar (
+      CFML.SepBase.SepBasicSetup.HS.repr (Dyn_array a) _prog_a
+    ) (
+      CFML.SepBase.SepBasicSetup.SepSimplArgsCredits.hstar (
+        CFML.SepBase.SepBasicSetup.HS.repr (Int n) _prog_n
+      ) (CFML.SepBase.SepBasicSetup.SepSimplArgsCredits.hpure (ge n (0)%Z))
+    )
+  ) (
+    fun _ : Coq.Init.Datatypes.unit =>
+    CFML.SepBase.SepBasicSetup.SepSimplArgsCredits.hexists (
+      fun _a_ : sequence int =>
+      CFML.SepBase.SepBasicSetup.SepSimplArgsCredits.hstar (
+        CFML.SepBase.SepBasicSetup.HS.repr (Dyn_array _a_) _prog_a
+      ) (
+        CFML.SepBase.SepBasicSetup.SepSimplArgsCredits.hstar (
+          CFML.SepBase.SepBasicSetup.HS.repr (Int n) _prog_n
+        ) (
+          CFML.SepBase.SepBasicSetup.SepSimplArgsCredits.hstar (
+            CFML.SepBase.SepBasicSetup.SepSimplArgsCredits.hpure (
+              ge n (length _a_) -> Coq.Init.Logic.eq _a_ a
+            )
+          ) (
+            CFML.SepBase.SepBasicSetup.SepSimplArgsCredits.hpure (
+              lt n (length _a_) -> Coq.Init.Logic.eq _a_ (seq_sub_r a n)
+            )
+          )
+        )
+      )
+    )
+  ).
+
+Parameter _clear : CFML.Semantics.val.
+
+Parameter _clear_spec :
+  forall _prog_a : loc,
+  forall a : sequence int,
+  CFML.SepLifted.Triple (
+    CFML.SepLifted.Trm_apps _clear (
+      Coq.Lists.List.cons (@CFML.SepLifted.dyn_make loc _ _prog_a) Coq.Lists.List.nil
+    )
+  ) (CFML.SepBase.SepBasicSetup.HS.repr (Dyn_array a) _prog_a) (
+    fun _ : Coq.Init.Datatypes.unit =>
+    CFML.SepBase.SepBasicSetup.HS.repr (Dyn_array empty) _prog_a
+  ).
