examples/translations/Epic/epic_mli.v
@@ -1,0 +1,26 @@
+Set Implicit Arguments.
+
+Require Import gospelstdlib_verified.
+
+Require Coq.ZArith.BinInt TLC.LibLogic TLC.LibRelation TLC.LibInt TLC.LibListZ.
+
+Require Import CFML.SepBase CFML.SepLifted CFML.WPLib CFML.WPLifted CFML.WPRecord CFML.WPArray CFML.WPBuiltin.
+
+Require CFML.Stdlib.Array_ml CFML.Stdlib.List_ml CFML.Stdlib.Sys_ml.
+
+Require Import Coq.ZArith.BinIntDef CFML.Semantics CFML.WPHeader.
+
+Delimit Scope Z_scope with Z.
+
+Axiom fold_left_cons :
+  forall {a44 : Type},
+  forall {a45 : Type},
+  forall {Ih_a44 : Inhab a44},
+  forall {Ih_a45 : Inhab a45},
+  forall f : sequence a45 -> a44 -> sequence a45,
+  forall acc : sequence a45,
+  forall x : a44,
+  forall l : sequence a44,
+  eq (fold_left f acc (cons x l)) (@empty a45 Ih_a45).
+
+
