examples/translations/Hashtbl/hashtbl_mli.v
@@ -1,0 +1,283 @@
+Set Implicit Arguments.
+
+Require Import gospelstdlib_verified.
+
+Require Coq.ZArith.BinInt TLC.LibLogic TLC.LibRelation TLC.LibInt TLC.LibListZ.
+
+Require Import CFML.SepBase CFML.SepLifted CFML.WPLib CFML.WPLifted CFML.WPRecord CFML.WPArray CFML.WPBuiltin.
+
+Require CFML.Stdlib.Array_ml CFML.Stdlib.List_ml CFML.Stdlib.Sys_ml.
+
+Require Import Coq.ZArith.BinIntDef CFML.Semantics CFML.WPHeader.
+
+Delimit Scope Z_scope with Z.
+
+Import Stdlib.
+
+Import Gospelstdlib.
+
+Import Sequence.
+
+Import Map.
+
+Parameter Hashtbl :
+  (int -> sequence int) ->
+  loc -> CFML.SepBase.SepBasicSetup.SepSimplArgsCredits.hprop.
+
+Parameter _create : CFML.Semantics.val.
+
+Parameter _create_spec :
+  forall n : int,
+  CFML.SepLifted.Triple (
+    CFML.SepLifted.Trm_apps _create (
+      Coq.Lists.List.cons (@CFML.SepLifted.dyn_make int _ n) Coq.Lists.List.nil
+    )
+  ) CFML.SepBase.SepBasicSetup.SepSimplArgsCredits.hempty (
+    fun _res_ : loc =>
+    let '(_prog_tbl) := _res_ in
+    CFML.SepBase.SepBasicSetup.HS.repr (Hashtbl (fun _ : int => empty)) _prog_tbl
+  ).
+
+Parameter _clear : CFML.Semantics.val.
+
+Parameter _clear_spec :
+  forall _prog_tbl : loc,
+  forall tbl : int -> sequence int,
+  CFML.SepLifted.Triple (
+    CFML.SepLifted.Trm_apps _clear (
+      Coq.Lists.List.cons (@CFML.SepLifted.dyn_make loc _ _prog_tbl) Coq.Lists.List.nil
+    )
+  ) (CFML.SepBase.SepBasicSetup.HS.repr (Hashtbl tbl) _prog_tbl) (
+    fun _res_ : Coq.Init.Datatypes.unit =>
+    CFML.SepBase.SepBasicSetup.SepSimplArgsCredits.hstar (
+      CFML.SepBase.SepBasicSetup.HS.repr (Hashtbl tbl) _prog_tbl
+    ) (
+      CFML.SepBase.SepBasicSetup.SepSimplArgsCredits.hpure (
+        Coq.Init.Logic.eq tbl (fun _ : int => empty)
+      )
+    )
+  ).
+
+Parameter _copy : CFML.Semantics.val.
+
+Parameter _copy_spec :
+  forall _prog_tbl : loc,
+  forall tbl : int -> sequence int,
+  CFML.SepLifted.Triple (
+    CFML.SepLifted.Trm_apps _copy (
+      Coq.Lists.List.cons (@CFML.SepLifted.dyn_make loc _ _prog_tbl) Coq.Lists.List.nil
+    )
+  ) (CFML.SepBase.SepBasicSetup.HS.repr (Hashtbl tbl) _prog_tbl) (
+    fun _res_ : loc =>
+    let '(_prog_c) := _res_ in
+    CFML.SepBase.SepBasicSetup.SepSimplArgsCredits.hexists (
+      fun c : int -> sequence int =>
+      CFML.SepBase.SepBasicSetup.SepSimplArgsCredits.hstar (
+        CFML.SepBase.SepBasicSetup.HS.repr (Hashtbl tbl) _prog_tbl
+      ) (
+        CFML.SepBase.SepBasicSetup.SepSimplArgsCredits.hstar (
+          CFML.SepBase.SepBasicSetup.HS.repr (Hashtbl c) _prog_c
+        ) (
+          CFML.SepBase.SepBasicSetup.SepSimplArgsCredits.hpure (
+            forall k : int,
+            Coq.Init.Logic.eq (tbl k) (c k)
+          )
+        )
+      )
+    )
+  ).
+
+Parameter _add : CFML.Semantics.val.
+
+Parameter _add_spec :
+  forall _prog_tbl : loc,
+  forall tbl : int -> sequence int,
+  forall k : int,
+  forall v : int,
+  CFML.SepLifted.Triple (
+    CFML.SepLifted.Trm_apps _add (
+      Coq.Lists.List.cons (@CFML.SepLifted.dyn_make loc _ _prog_tbl) (
+        Coq.Lists.List.cons (@CFML.SepLifted.dyn_make int _ k) (
+          Coq.Lists.List.cons (@CFML.SepLifted.dyn_make int _ v) Coq.Lists.List.nil
+        )
+      )
+    )
+  ) (CFML.SepBase.SepBasicSetup.HS.repr (Hashtbl tbl) _prog_tbl) (
+    fun _res_ : Coq.Init.Datatypes.unit =>
+    CFML.SepBase.SepBasicSetup.HS.repr (
+      Hashtbl (map_set tbl k (cons v (tbl k)))
+    ) _prog_tbl
+  ).
+
+Parameter _find_opt : CFML.Semantics.val.
+
+Parameter _find_opt_spec :
+  forall _prog_tbl : loc,
+  forall tbl : int -> sequence int,
+  forall k : int,
+  CFML.SepLifted.Triple (
+    CFML.SepLifted.Trm_apps _find_opt (
+      Coq.Lists.List.cons (@CFML.SepLifted.dyn_make loc _ _prog_tbl) (
+        Coq.Lists.List.cons (@CFML.SepLifted.dyn_make int _ k) Coq.Lists.List.nil
+      )
+    )
+  ) (CFML.SepBase.SepBasicSetup.HS.repr (Hashtbl tbl) _prog_tbl) (
+    fun _res_ : option int =>
+    let '(r) := _res_ in
+    CFML.SepBase.SepBasicSetup.SepSimplArgsCredits.hstar (
+      CFML.SepBase.SepBasicSetup.HS.repr (Hashtbl tbl) _prog_tbl
+    ) (
+      CFML.SepBase.SepBasicSetup.SepSimplArgsCredits.hpure (
+        match r with
+        | None => Coq.Init.Logic.eq (tbl k) empty
+          | Some x => Coq.Init.Logic.eq (hd (tbl k)) x
+          end
+      )
+    )
+  ).
+
+Parameter _find_all : CFML.Semantics.val.
+
+Parameter _find_all_spec :
+  forall _prog_tbl : loc,
+  forall tbl : int -> sequence int,
+  forall k : int,
+  CFML.SepLifted.Triple (
+    CFML.SepLifted.Trm_apps _find_all (
+      Coq.Lists.List.cons (@CFML.SepLifted.dyn_make loc _ _prog_tbl) (
+        Coq.Lists.List.cons (@CFML.SepLifted.dyn_make int _ k) Coq.Lists.List.nil
+      )
+    )
+  ) (CFML.SepBase.SepBasicSetup.HS.repr (Hashtbl tbl) _prog_tbl) (
+    fun _res_ : list int =>
+    let '(l) := _res_ in
+    CFML.SepBase.SepBasicSetup.SepSimplArgsCredits.hstar (
+      CFML.SepBase.SepBasicSetup.HS.repr (Hashtbl tbl) _prog_tbl
+    ) (
+      CFML.SepBase.SepBasicSetup.SepSimplArgsCredits.hpure (
+        Coq.Init.Logic.eq (of_list l) (tbl k)
+      )
+    )
+  ).
+
+Parameter _mem : CFML.Semantics.val.
+
+Parameter _mem_spec :
+  forall _prog_tbl : loc,
+  forall tbl : int -> sequence int,
+  forall k : int,
+  CFML.SepLifted.Triple (
+    CFML.SepLifted.Trm_apps _mem (
+      Coq.Lists.List.cons (@CFML.SepLifted.dyn_make loc _ _prog_tbl) (
+        Coq.Lists.List.cons (@CFML.SepLifted.dyn_make int _ k) Coq.Lists.List.nil
+      )
+    )
+  ) (CFML.SepBase.SepBasicSetup.HS.repr (Hashtbl tbl) _prog_tbl) (
+    fun _res_ : bool =>
+    let '(b) := _res_ in
+    CFML.SepBase.SepBasicSetup.SepSimplArgsCredits.hstar (
+      CFML.SepBase.SepBasicSetup.HS.repr (Hashtbl tbl) _prog_tbl
+    ) (
+      CFML.SepBase.SepBasicSetup.SepSimplArgsCredits.hpure (
+        Coq.Init.Logic.iff b (
+          Coq.Init.Logic.not (Coq.Init.Logic.eq (tbl k) empty)
+        )
+      )
+    )
+  ).
+
+Parameter _remove : CFML.Semantics.val.
+
+Parameter _remove_spec :
+  forall _prog_tbl : loc,
+  forall tbl : int -> sequence int,
+  forall k : int,
+  CFML.SepLifted.Triple (
+    CFML.SepLifted.Trm_apps _remove (
+      Coq.Lists.List.cons (@CFML.SepLifted.dyn_make loc _ _prog_tbl) (
+        Coq.Lists.List.cons (@CFML.SepLifted.dyn_make int _ k) Coq.Lists.List.nil
+      )
+    )
+  ) (CFML.SepBase.SepBasicSetup.HS.repr (Hashtbl tbl) _prog_tbl) (
+    fun _res_ : Coq.Init.Datatypes.unit =>
+    CFML.SepBase.SepBasicSetup.SepSimplArgsCredits.hexists (
+      fun _tbl_ : int -> sequence int =>
+      CFML.SepBase.SepBasicSetup.SepSimplArgsCredits.hstar (
+        CFML.SepBase.SepBasicSetup.HS.repr (Hashtbl _tbl_) _prog_tbl
+      ) (
+        CFML.SepBase.SepBasicSetup.SepSimplArgsCredits.hstar (
+          CFML.SepBase.SepBasicSetup.SepSimplArgsCredits.hpure (
+            Coq.Init.Logic.eq (tbl k) empty -> Coq.Init.Logic.eq _tbl_ tbl
+          )
+        ) (
+          CFML.SepBase.SepBasicSetup.SepSimplArgsCredits.hpure (
+            Coq.Init.Logic.not (Coq.Init.Logic.eq (_tbl_ k) empty) ->
+            Coq.Init.Logic.eq _tbl_ (map_set tbl k (tl (tbl k)))
+          )
+        )
+      )
+    )
+  ).
+
+Parameter _replace : CFML.Semantics.val.
+
+Parameter _replace_spec :
+  forall _prog_tbl : loc,
+  forall tbl : int -> sequence int,
+  forall k : int,
+  forall v : int,
+  CFML.SepLifted.Triple (
+    CFML.SepLifted.Trm_apps _replace (
+      Coq.Lists.List.cons (@CFML.SepLifted.dyn_make loc _ _prog_tbl) (
+        Coq.Lists.List.cons (@CFML.SepLifted.dyn_make int _ k) (
+          Coq.Lists.List.cons (@CFML.SepLifted.dyn_make int _ v) Coq.Lists.List.nil
+        )
+      )
+    )
+  ) (CFML.SepBase.SepBasicSetup.HS.repr (Hashtbl tbl) _prog_tbl) (
+    fun _res_ : Coq.Init.Datatypes.unit =>
+    CFML.SepBase.SepBasicSetup.SepSimplArgsCredits.hexists (
+      fun _tbl_ : int -> sequence int =>
+      CFML.SepBase.SepBasicSetup.SepSimplArgsCredits.hstar (
+        CFML.SepBase.SepBasicSetup.HS.repr (Hashtbl _tbl_) _prog_tbl
+      ) (
+        CFML.SepBase.SepBasicSetup.SepSimplArgsCredits.hstar (
+          CFML.SepBase.SepBasicSetup.SepSimplArgsCredits.hpure (
+            Coq.Init.Logic.eq (_tbl_ k) empty ->
+            Coq.Init.Logic.eq _tbl_ (map_set _tbl_ k (singleton v))
+          )
+        ) (
+          CFML.SepBase.SepBasicSetup.SepSimplArgsCredits.hpure (
+            Coq.Init.Logic.not (Coq.Init.Logic.eq (_tbl_ k) empty) ->
+            (
+              let '(tail) := tl (tbl k) in
+              Coq.Init.Logic.eq _tbl_ (map_set tbl k (cons v tail))
+            )
+          )
+        )
+      )
+    )
+  ).
+
+Parameter _length : CFML.Semantics.val.
+
+Parameter _length_spec :
+  forall _prog_tbl : loc,
+  forall tbl : int -> sequence int,
+  CFML.SepLifted.Triple (
+    CFML.SepLifted.Trm_apps _length (
+      Coq.Lists.List.cons (@CFML.SepLifted.dyn_make loc _ _prog_tbl) Coq.Lists.List.nil
+    )
+  ) (CFML.SepBase.SepBasicSetup.HS.repr (Hashtbl tbl) _prog_tbl) (
+    fun _res_ : int =>
+    let '(n) := _res_ in
+    CFML.SepBase.SepBasicSetup.SepSimplArgsCredits.hstar (
+      CFML.SepBase.SepBasicSetup.HS.repr (Hashtbl tbl) _prog_tbl
+    ) (
+      CFML.SepBase.SepBasicSetup.SepSimplArgsCredits.hpure (
+        Coq.Init.Logic.eq n (_Set.cardinal (domain empty tbl))
+      )
+    )
+  ).
+
+
