examples/translations/Mem_stack/mem_stack_mli.v
@@ -1,0 +1,214 @@
+Set Implicit Arguments.
+
+Require Import gospelstdlib_verified.
+
+Require Coq.ZArith.BinInt TLC.LibLogic TLC.LibRelation TLC.LibInt TLC.LibListZ.
+
+Require Import CFML.SepBase CFML.SepLifted CFML.WPLib CFML.WPLifted CFML.WPRecord CFML.WPArray CFML.WPBuiltin.
+
+Require CFML.Stdlib.Array_ml CFML.Stdlib.List_ml CFML.Stdlib.Sys_ml.
+
+Require Import Coq.ZArith.BinIntDef CFML.Semantics CFML.WPHeader.
+
+Delimit Scope Z_scope with Z.
+
+Import Stdlib.
+
+Import Gospelstdlib.
+
+Parameter Estack :
+  forall {a : Type},
+  forall {Ih_a : Inhab a},
+  forall {Enc_a : Enc a},
+  sequence a ->
+  loc -> CFML.SepBase.SepBasicSetup.SepSimplArgsCredits.hprop.
+
+Parameter _ecreate : CFML.Semantics.val.
+
+Parameter _ecreate_spec :
+  forall {a : Type},
+  forall {Ih_a : Inhab a},
+  forall {Enc_a : Enc a},
+  forall x : a,
+  CFML.SepLifted.Triple (
+    CFML.SepLifted.Trm_apps _ecreate (
+      Coq.Lists.List.cons (@CFML.SepLifted.dyn_make a _ x) Coq.Lists.List.nil
+    )
+  ) CFML.SepBase.SepBasicSetup.SepSimplArgsCredits.hempty (
+    fun _res_ : loc =>
+    let '(_prog_r) := _res_ in
+    CFML.SepBase.SepBasicSetup.HS.repr (Estack (@Sequence.empty a Ih_a)) _prog_r
+  ).
+
+Parameter _epush : CFML.Semantics.val.
+
+Parameter _epush_spec :
+  forall {a : Type},
+  forall {Ih_a : Inhab a},
+  forall {Enc_a : Enc a},
+  forall _prog_s : loc,
+  forall s : sequence a,
+  forall x : a,
+  CFML.SepLifted.Triple (
+    CFML.SepLifted.Trm_apps _epush (
+      Coq.Lists.List.cons (@CFML.SepLifted.dyn_make loc _ _prog_s) (
+        Coq.Lists.List.cons (@CFML.SepLifted.dyn_make a _ x) Coq.Lists.List.nil
+      )
+    )
+  ) (CFML.SepBase.SepBasicSetup.HS.repr (Estack s) _prog_s) (
+    fun _res_ : Coq.Init.Datatypes.unit =>
+    CFML.SepBase.SepBasicSetup.HS.repr (Estack (Sequence.cons x s)) _prog_s
+  ).
+
+Parameter _epop : CFML.Semantics.val.
+
+Parameter _epop_spec :
+  forall {a : Type},
+  forall {Ih_a : Inhab a},
+  forall {Enc_a : Enc a},
+  forall _prog_s : loc,
+  forall s : sequence a,
+  CFML.SepLifted.Triple (
+    CFML.SepLifted.Trm_apps _epop (
+      Coq.Lists.List.cons (@CFML.SepLifted.dyn_make loc _ _prog_s) Coq.Lists.List.nil
+    )
+  ) (
+    CFML.SepBase.SepBasicSetup.SepSimplArgsCredits.hstar (
+      CFML.SepBase.SepBasicSetup.HS.repr (Estack s) _prog_s
+    ) (
+      CFML.SepBase.SepBasicSetup.SepSimplArgsCredits.hpure (
+        Coq.Init.Logic.not (Coq.Init.Logic.eq s (@Sequence.empty a Ih_a))
+      )
+    )
+  ) (
+    fun _res_ : a =>
+    let '(r) := _res_ in
+    CFML.SepBase.SepBasicSetup.SepSimplArgsCredits.hexists (
+      fun _s_ : sequence a =>
+      CFML.SepBase.SepBasicSetup.SepSimplArgsCredits.hstar (
+        CFML.SepBase.SepBasicSetup.HS.repr (Estack _s_) _prog_s
+      ) (
+        CFML.SepBase.SepBasicSetup.SepSimplArgsCredits.hpure (
+          Coq.Init.Logic.eq s (Sequence.cons r _s_)
+        )
+      )
+    )
+  ).
+
+Parameter pstack : Type -> Type.
+
+Parameter _pcreate : CFML.Semantics.val.
+
+Parameter _pcreate_spec :
+  forall {a : Type},
+  forall {Ih_a : Inhab a},
+  forall {Enc_a : Enc a},
+  forall x : a,
+  CFML.SepLifted.Triple (
+    CFML.SepLifted.Trm_apps _pcreate (
+      Coq.Lists.List.cons (@CFML.SepLifted.dyn_make a _ x) Coq.Lists.List.nil
+    )
+  ) CFML.SepBase.SepBasicSetup.SepSimplArgsCredits.hempty (
+    fun _res_ : pstack a =>
+    let '(_prog_r) := _res_ in
+    CFML.SepBase.SepBasicSetup.HS.repr (Pstack (@Sequence.empty a Ih_a)) _prog_r
+  ).
+
+Parameter _ppush : CFML.Semantics.val.
+
+Parameter _ppush_spec :
+  forall {a : Type},
+  forall {Ih_a : Inhab a},
+  forall {Enc_a : Enc a},
+  forall _prog_s : pstack a,
+  forall s : sequence a,
+  forall x : a,
+  CFML.SepLifted.Triple (
+    CFML.SepLifted.Trm_apps _ppush (
+      Coq.Lists.List.cons (@CFML.SepLifted.dyn_make (pstack a) _ _prog_s) (
+        Coq.Lists.List.cons (@CFML.SepLifted.dyn_make a _ x) Coq.Lists.List.nil
+      )
+    )
+  ) (CFML.SepBase.SepBasicSetup.HS.repr (Pstack s) _prog_s) (
+    fun _res_ : pstack a =>
+    let '(_prog_r) := _res_ in
+    CFML.SepBase.SepBasicSetup.SepSimplArgsCredits.hexists (
+      fun _s_ : sequence a =>
+      CFML.SepBase.SepBasicSetup.SepSimplArgsCredits.hstar (
+        CFML.SepBase.SepBasicSetup.HS.repr (Pstack _s_) _prog_s
+      ) (
+        CFML.SepBase.SepBasicSetup.HS.repr (Pstack (Sequence.cons x _s_)) _prog_r
+      )
+    )
+  ).
+
+Parameter _ppop : CFML.Semantics.val.
+
+Parameter _ppop_spec :
+  forall {a : Type},
+  forall {Ih_a : Inhab a},
+  forall {Enc_a : Enc a},
+  forall _prog_s : pstack a,
+  forall s : sequence a,
+  CFML.SepLifted.Triple (
+    CFML.SepLifted.Trm_apps _ppop (
+      Coq.Lists.List.cons (@CFML.SepLifted.dyn_make (pstack a) _ _prog_s) Coq.Lists.List.nil
+    )
+  ) (
+    CFML.SepBase.SepBasicSetup.SepSimplArgsCredits.hstar (
+      CFML.SepBase.SepBasicSetup.HS.repr (Pstack s) _prog_s
+    ) (
+      CFML.SepBase.SepBasicSetup.SepSimplArgsCredits.hpure (
+        Coq.Init.Logic.not (Coq.Init.Logic.eq s (@Sequence.empty a Ih_a))
+      )
+    )
+  ) (
+    fun _res_ : Coq.Init.Datatypes.prod (pstack a) a =>
+    let '(_prog_rs, res) := _res_ in
+    CFML.SepBase.SepBasicSetup.SepSimplArgsCredits.hexists (
+      fun rs : sequence a =>
+      CFML.SepBase.SepBasicSetup.SepSimplArgsCredits.hstar (
+        CFML.SepBase.SepBasicSetup.HS.repr (Pstack (Sequence.cons res rs)) _prog_s
+      ) (CFML.SepBase.SepBasicSetup.HS.repr (Pstack rs) _prog_rs)
+    )
+  ).
+
+Parameter _pstack_to_estack : CFML.Semantics.val.
+
+Parameter _pstack_to_estack_spec :
+  forall {a : Type},
+  forall {Ih_a : Inhab a},
+  forall {Enc_a : Enc a},
+  forall _prog_ps : pstack a,
+  forall ps : sequence a,
+  CFML.SepLifted.Triple (
+    CFML.SepLifted.Trm_apps _pstack_to_estack (
+      Coq.Lists.List.cons (@CFML.SepLifted.dyn_make (pstack a) _ _prog_ps) Coq.Lists.List.nil
+    )
+  ) (CFML.SepBase.SepBasicSetup.HS.repr (Pstack ps) _prog_ps) (
+    fun _res_ : loc =>
+    let '(_prog_re) := _res_ in
+    CFML.SepBase.SepBasicSetup.SepSimplArgsCredits.hstar (
+      CFML.SepBase.SepBasicSetup.HS.repr (Pstack ps) _prog_ps
+    ) (CFML.SepBase.SepBasicSetup.HS.repr (Estack ps) _prog_re)
+  ).
+
+Parameter _estack_to_pstack : CFML.Semantics.val.
+
+Parameter _estack_to_pstack_spec :
+  forall {a : Type},
+  forall {Ih_a : Inhab a},
+  forall {Enc_a : Enc a},
+  forall _prog_es : loc,
+  forall es : sequence a,
+  CFML.SepLifted.Triple (
+    CFML.SepLifted.Trm_apps _estack_to_pstack (
+      Coq.Lists.List.cons (@CFML.SepLifted.dyn_make loc _ _prog_es) Coq.Lists.List.nil
+    )
+  ) (CFML.SepBase.SepBasicSetup.HS.repr (Estack es) _prog_es) (
+    fun _res_ : pstack a =>
+    let '(_prog_rp) := _res_ in
+    CFML.SepBase.SepBasicSetup.HS.repr (Pstack es) _prog_rp
+  ).
+
+
