examples/translations/Mem_stack_memory/mem_stack_memory_mli.v
@@ -1,0 +1,449 @@
+Set Implicit Arguments.
+
+Require Import gospelstdlib_verified.
+Require Coq.ZArith.BinInt TLC.LibLogic TLC.LibRelation TLC.LibInt TLC.LibListZ.
+
+Require Import CFML.SepBase CFML.SepLifted CFML.WPLib CFML.WPLifted CFML.WPRecord CFML.WPArray CFML.WPBuiltin.
+
+Require CFML.Stdlib.Array_ml CFML.Stdlib.List_ml CFML.Stdlib.Sys_ml.
+
+Require Import Coq.ZArith.BinIntDef CFML.Semantics CFML.WPHeader.
+
+Delimit Scope Z_scope with Z.
+
+Import Stdlib.
+
+Import Gospelstdlib.
+
+Parameter memory : Type -> Type.
+
+Parameter __Enc_memory : forall a : Type, CFML.SepLifted.Enc (memory a).
+
+Instance _Enc_memory : forall a : Type, CFML.SepLifted.Enc (memory a) :=
+__Enc_memory.
+
+Parameter Memory :
+  forall a : Type,
+  forall {Ea : OCamlType a},
+  memory a ->
+  memory a -> CFML.SepBase.SepBasicSetup.SepSimplArgsCredits.hprop.
+
+Parameter extend :
+  forall a : Type,
+  forall {aIh : OCamlType a},
+  memory a -> memory a -> Prop.
+
+Parameter refl :
+  forall a : Type,
+  forall {aIh : OCamlType a},
+  CFML.SepBase.SepBasicSetup.SepSimplArgsCredits.himpl CFML.SepBase.SepBasicSetup.SepSimplArgsCredits.hempty (
+    CFML.SepBase.SepBasicSetup.SepSimplArgsCredits.hforall (
+      fun m : memory a =>
+      CFML.SepBase.SepBasicSetup.SepSimplArgsCredits.hpure (extend m m)
+    )
+  ).
+
+Parameter tran :
+  forall a : Type,
+  forall {aIh : OCamlType a},
+  CFML.SepBase.SepBasicSetup.SepSimplArgsCredits.himpl CFML.SepBase.SepBasicSetup.SepSimplArgsCredits.hempty (
+    CFML.SepBase.SepBasicSetup.SepSimplArgsCredits.hforall (
+      fun m1 : memory a =>
+      CFML.SepBase.SepBasicSetup.SepSimplArgsCredits.hforall (
+        fun m2 : memory a =>
+        CFML.SepBase.SepBasicSetup.SepSimplArgsCredits.hforall (
+          fun m3 : memory a =>
+          CFML.SepBase.SepBasicSetup.SepSimplArgsCredits.hpure (
+            extend m1 m2 -> extend m2 m3 -> extend m1 m3
+          )
+        )
+      )
+    )
+  ).
+
+Parameter _create_mem : CFML.Semantics.val.
+
+Parameter _create_mem_spec :
+  forall a : Type,
+  forall {aIh : Inhab a},
+  forall {Ea : CFML.SepLifted.Enc a},
+  CFML.SepLifted.Triple (
+    CFML.SepLifted.Trm_apps _create_mem (
+      Coq.Lists.List.cons (
+        @CFML.SepLifted.dyn_make CFML.Semantics.val _ Coq.Init.Datatypes.tt
+      ) Coq.Lists.List.nil
+    )
+  ) CFML.SepBase.SepBasicSetup.SepSimplArgsCredits.hempty (
+    fun _res_ : memory a =>
+    let '(result) := _res_ in
+    CFML.SepBase.SepBasicSetup.SepSimplArgsCredits.hempty
+  ).
+
+Lemma Estack :
+  forall a : Type,
+  forall {aIh : OCamlType a},
+  (memory a -> sequence a) ->
+  loc -> CFML.SepBase.SepBasicSetup.SepSimplArgsCredits.hprop.
+Admitted.
+
+Lemma estack_mon :
+  forall a : Type,
+  forall {aIh : OCamlType a},
+  CFML.SepBase.SepBasicSetup.SepSimplArgsCredits.himpl CFML.SepBase.SepBasicSetup.SepSimplArgsCredits.hempty (
+    CFML.SepBase.SepBasicSetup.SepSimplArgsCredits.hforall (
+      fun m : memory a =>
+      CFML.SepBase.SepBasicSetup.SepSimplArgsCredits.hforall (
+        fun m' : memory a =>
+        CFML.SepBase.SepBasicSetup.SepSimplArgsCredits.hforall (
+          fun _prog_e : loc =>
+          CFML.SepBase.SepBasicSetup.SepSimplArgsCredits.hforall (
+            fun e : memory a -> sequence a =>
+            CFML.SepBase.SepBasicSetup.SepSimplArgsCredits.hwand (
+              CFML.SepBase.SepBasicSetup.HS.repr (Estack e) _prog_e
+            ) (
+              CFML.SepBase.SepBasicSetup.SepSimplArgsCredits.hstar (
+                CFML.SepBase.SepBasicSetup.HS.repr (Estack e) _prog_e
+              ) (
+                CFML.SepBase.SepBasicSetup.SepSimplArgsCredits.hpure (
+                  extend m m' -> Coq.Init.Logic.eq (e m) (e m')
+                )
+              )
+            )
+          )
+        )
+      )
+    )
+  ).
+
+Parameter _ecreate : CFML.Semantics.val.
+
+Parameter _ecreate_spec :
+  forall a : Type,
+  forall {aIh : OCamlType a},
+  forall m : memory a,
+  forall x : a,
+  CFML.SepLifted.Triple (
+    CFML.SepLifted.Trm_apps _ecreate (
+      Coq.Lists.List.cons (@CFML.SepLifted.dyn_make (memory a) _ m) (
+        Coq.Lists.List.cons (@CFML.SepLifted.dyn_make a _ x) Coq.Lists.List.nil
+      )
+    )
+  ) CFML.SepBase.SepBasicSetup.SepSimplArgsCredits.hempty (
+    fun _res_ : loc =>
+    let '(_prog_r) := _res_ in
+    CFML.SepBase.SepBasicSetup.SepSimplArgsCredits.hexists (
+      fun r : memory a -> sequence a =>
+      CFML.SepBase.SepBasicSetup.SepSimplArgsCredits.hstar (
+        CFML.SepBase.SepBasicSetup.HS.repr (Estack r) _prog_r
+      ) (
+        CFML.SepBase.SepBasicSetup.SepSimplArgsCredits.hpure (
+          Coq.Init.Logic.eq (r m) (@Sequence.empty a _G)
+        )
+      )
+    )
+  ).
+
+Parameter _epush : CFML.Semantics.val.
+
+Parameter _epush_spec :
+  forall a : Type,
+  forall {aIh : OCamlType a},
+  forall {Ea : CFML.SepLifted.Enc a},
+  forall m : memory a,
+  forall _prog_s : loc,
+  forall s : memory a -> sequence a,
+  forall x : a,
+  CFML.SepLifted.Triple (
+    CFML.SepLifted.Trm_apps _epush (
+      Coq.Lists.List.cons (@CFML.SepLifted.dyn_make (memory a) _ m) (
+        Coq.Lists.List.cons (@CFML.SepLifted.dyn_make loc _ _prog_s) (
+          Coq.Lists.List.cons (@CFML.SepLifted.dyn_make a _ x) Coq.Lists.List.nil
+        )
+      )
+    )
+  ) (CFML.SepBase.SepBasicSetup.HS.repr (Estack s) _prog_s) (
+    fun _res_ : Coq.Init.Datatypes.unit =>
+    CFML.SepBase.SepBasicSetup.SepSimplArgsCredits.hexists (
+      fun _s_ : memory a -> sequence a =>
+      CFML.SepBase.SepBasicSetup.SepSimplArgsCredits.hstar (
+        CFML.SepBase.SepBasicSetup.HS.repr (Estack _s_) _prog_s
+      ) (
+        CFML.SepBase.SepBasicSetup.SepSimplArgsCredits.hpure (
+          Coq.Init.Logic.eq (_s_ m) (Sequence.cons x (s m))
+        )
+      )
+    )
+  ).
+
+Parameter _epop : CFML.Semantics.val.
+
+Parameter _epop_spec :
+  forall a : Type,
+  forall {aIh : OCamlType a},
+  forall {Ea : CFML.SepLifted.Enc a},
+  forall m : memory a,
+  forall _prog_s : loc,
+  forall s : memory a -> sequence a,
+  CFML.SepLifted.Triple (
+    CFML.SepLifted.Trm_apps _epop (
+      Coq.Lists.List.cons (@CFML.SepLifted.dyn_make (memory a) _ m) (
+        Coq.Lists.List.cons (@CFML.SepLifted.dyn_make loc _ _prog_s) Coq.Lists.List.nil
+      )
+    )
+  ) (
+    CFML.SepBase.SepBasicSetup.SepSimplArgsCredits.hstar (
+      CFML.SepBase.SepBasicSetup.HS.repr (Estack s) _prog_s
+    ) (
+      CFML.SepBase.SepBasicSetup.SepSimplArgsCredits.hpure (
+        Coq.Init.Logic.not (Coq.Init.Logic.eq (s m) (@Sequence.empty a _G))
+      )
+    )
+  ) (
+    fun _res_ : a =>
+    let '(r) := _res_ in
+    CFML.SepBase.SepBasicSetup.SepSimplArgsCredits.hexists (
+      fun _s_ : memory a -> sequence a =>
+      CFML.SepBase.SepBasicSetup.SepSimplArgsCredits.hstar (
+        CFML.SepBase.SepBasicSetup.HS.repr (Estack _s_) _prog_s
+      ) (
+        CFML.SepBase.SepBasicSetup.SepSimplArgsCredits.hpure (
+          Coq.Init.Logic.eq (s m) (Sequence.cons r (_s_ m))
+        )
+      )
+    )
+  ).
+
+Record pstack (a : Type) : Type := _mk_pstack {
+  internal : unit;
+  pview : memory a -> sequence a
+}.
+
+Parameter Pstack :
+  forall a : Type,
+  forall {aIh : Inhab a},
+  forall {Ea : CFML.SepLifted.Enc a},
+  pstack a -> loc -> CFML.SepBase.SepBasicSetup.SepSimplArgsCredits.hprop.
+
+Parameter pstack_mon :
+  forall a : Type,
+  forall {aIh : Inhab a},
+  forall {Ea : CFML.SepLifted.Enc a},
+  CFML.SepBase.SepBasicSetup.SepSimplArgsCredits.himpl CFML.SepBase.SepBasicSetup.SepSimplArgsCredits.hempty (
+    CFML.SepBase.SepBasicSetup.SepSimplArgsCredits.hforall (
+      fun m : memory a =>
+      CFML.SepBase.SepBasicSetup.SepSimplArgsCredits.hforall (
+        fun m' : memory a =>
+        CFML.SepBase.SepBasicSetup.SepSimplArgsCredits.hforall (
+          fun _prog_p : loc =>
+          CFML.SepBase.SepBasicSetup.SepSimplArgsCredits.hforall (
+            fun p : pstack a =>
+            CFML.SepBase.SepBasicSetup.SepSimplArgsCredits.hwand (
+              CFML.SepBase.SepBasicSetup.HS.repr (Pstack p) _prog_p
+            ) (
+              CFML.SepBase.SepBasicSetup.SepSimplArgsCredits.hstar (
+                CFML.SepBase.SepBasicSetup.HS.repr (Pstack p) _prog_p
+              ) (
+                CFML.SepBase.SepBasicSetup.SepSimplArgsCredits.hpure (
+                  extend m m' -> Coq.Init.Logic.eq ((pview p) m) ((pview p) m')
+                )
+              )
+            )
+          )
+        )
+      )
+    )
+  ).
+
+Parameter _pcreate : CFML.Semantics.val.
+
+Parameter _pcreate_spec :
+  forall a : Type,
+  forall {aIh : Inhab a},
+  forall {Ea : CFML.SepLifted.Enc a},
+  forall m : memory a,
+  forall x : a,
+  CFML.SepLifted.Triple (
+    CFML.SepLifted.Trm_apps _pcreate (
+      Coq.Lists.List.cons (@CFML.SepLifted.dyn_make (memory a) _ m) (
+        Coq.Lists.List.cons (@CFML.SepLifted.dyn_make a _ x) Coq.Lists.List.nil
+      )
+    )
+  ) CFML.SepBase.SepBasicSetup.SepSimplArgsCredits.hempty (
+    fun _res_ : Coq.Init.Datatypes.prod loc (memory a) =>
+    let '(_prog_r, m') := _res_ in
+    CFML.SepBase.SepBasicSetup.SepSimplArgsCredits.hexists (
+      fun r : pstack a =>
+      CFML.SepBase.SepBasicSetup.SepSimplArgsCredits.hstar (
+        CFML.SepBase.SepBasicSetup.HS.repr (Pstack r) _prog_r
+      ) (
+        CFML.SepBase.SepBasicSetup.SepSimplArgsCredits.hstar (
+          CFML.SepBase.SepBasicSetup.SepSimplArgsCredits.hpure (
+            Coq.Init.Logic.eq ((pview r) m') (@Sequence.empty a aIh)
+          )
+        ) (CFML.SepBase.SepBasicSetup.SepSimplArgsCredits.hpure (extend m m'))
+      )
+    )
+  ).
+
+Parameter _ppush : CFML.Semantics.val.
+
+Parameter _ppush_spec :
+  forall a : Type,
+  forall {aIh : Inhab a},
+  forall {Ea : CFML.SepLifted.Enc a},
+  forall m : memory a,
+  forall _prog_s : loc,
+  forall s : pstack a,
+  forall x : a,
+  CFML.SepLifted.Triple (
+    CFML.SepLifted.Trm_apps _ppush (
+      Coq.Lists.List.cons (@CFML.SepLifted.dyn_make (memory a) _ m) (
+        Coq.Lists.List.cons (@CFML.SepLifted.dyn_make loc _ _prog_s) (
+          Coq.Lists.List.cons (@CFML.SepLifted.dyn_make a _ x) Coq.Lists.List.nil
+        )
+      )
+    )
+  ) (CFML.SepBase.SepBasicSetup.HS.repr (Pstack s) _prog_s) (
+    fun _res_ : Coq.Init.Datatypes.prod loc (memory a) =>
+    let '(_prog_r, m') := _res_ in
+    CFML.SepBase.SepBasicSetup.SepSimplArgsCredits.hexists (
+      fun _s_ : pstack a =>
+      CFML.SepBase.SepBasicSetup.SepSimplArgsCredits.hexists (
+        fun r : pstack a =>
+        CFML.SepBase.SepBasicSetup.SepSimplArgsCredits.hstar (
+          CFML.SepBase.SepBasicSetup.HS.repr (Pstack _s_) _prog_s
+        ) (
+          CFML.SepBase.SepBasicSetup.SepSimplArgsCredits.hstar (
+            CFML.SepBase.SepBasicSetup.HS.repr (Pstack r) _prog_r
+          ) (
+            CFML.SepBase.SepBasicSetup.SepSimplArgsCredits.hstar (
+              CFML.SepBase.SepBasicSetup.SepSimplArgsCredits.hpure (
+                Coq.Init.Logic.eq ((pview r) m') (
+                  Sequence.cons x ((pview _s_) m)
+                )
+              )
+            ) (
+              CFML.SepBase.SepBasicSetup.SepSimplArgsCredits.hpure (extend m m')
+            )
+          )
+        )
+      )
+    )
+  ).
+
+Parameter _ppop : CFML.Semantics.val.
+
+Parameter _ppop_spec :
+  forall a : Type,
+  forall {aIh : Inhab a},
+  forall {Ea : CFML.SepLifted.Enc a},
+  forall m : memory a,
+  forall _prog_s : loc,
+  forall s : pstack a,
+  CFML.SepLifted.Triple (
+    CFML.SepLifted.Trm_apps _ppop (
+      Coq.Lists.List.cons (@CFML.SepLifted.dyn_make (memory a) _ m) (
+        Coq.Lists.List.cons (@CFML.SepLifted.dyn_make loc _ _prog_s) Coq.Lists.List.nil
+      )
+    )
+  ) (
+    CFML.SepBase.SepBasicSetup.SepSimplArgsCredits.hstar (
+      CFML.SepBase.SepBasicSetup.HS.repr (Pstack s) _prog_s
+    ) (
+      CFML.SepBase.SepBasicSetup.SepSimplArgsCredits.hpure (
+        Coq.Init.Logic.not (
+          Coq.Init.Logic.eq ((pview s) m) (@Sequence.empty a aIh)
+        )
+      )
+    )
+  ) (
+    fun _res_ : Coq.Init.Datatypes.prod loc a =>
+    let '(_prog_rs, res) := _res_ in
+    CFML.SepBase.SepBasicSetup.SepSimplArgsCredits.hexists (
+      fun _s_ : pstack a =>
+      CFML.SepBase.SepBasicSetup.SepSimplArgsCredits.hexists (
+        fun rs : pstack a =>
+        CFML.SepBase.SepBasicSetup.SepSimplArgsCredits.hstar (
+          CFML.SepBase.SepBasicSetup.HS.repr (Pstack _s_) _prog_s
+        ) (
+          CFML.SepBase.SepBasicSetup.SepSimplArgsCredits.hstar (
+            CFML.SepBase.SepBasicSetup.HS.repr (Pstack rs) _prog_rs
+          ) (
+            CFML.SepBase.SepBasicSetup.SepSimplArgsCredits.hpure (
+              Coq.Init.Logic.eq ((pview _s_) m) (
+                Sequence.cons res ((pview rs) m)
+              )
+            )
+          )
+        )
+      )
+    )
+  ).
+
+Parameter _pstack_to_estack : CFML.Semantics.val.
+
+Parameter _pstack_to_estack_spec :
+  forall a : Type,
+  forall {aIh : Inhab a},
+  forall {Ea : CFML.SepLifted.Enc a},
+  forall m : memory a,
+  forall _prog_ps : loc,
+  forall ps : pstack a,
+  CFML.SepLifted.Triple (
+    CFML.SepLifted.Trm_apps _pstack_to_estack (
+      Coq.Lists.List.cons (@CFML.SepLifted.dyn_make (memory a) _ m) (
+        Coq.Lists.List.cons (@CFML.SepLifted.dyn_make loc _ _prog_ps) Coq.Lists.List.nil
+      )
+    )
+  ) (CFML.SepBase.SepBasicSetup.HS.repr (Pstack ps) _prog_ps) (
+    fun _res_ : loc =>
+    let '(_prog_re) := _res_ in
+    CFML.SepBase.SepBasicSetup.SepSimplArgsCredits.hexists (
+      fun re : memory a -> sequence a =>
+      CFML.SepBase.SepBasicSetup.SepSimplArgsCredits.hstar (
+        CFML.SepBase.SepBasicSetup.HS.repr (Pstack ps) _prog_ps
+      ) (
+        CFML.SepBase.SepBasicSetup.SepSimplArgsCredits.hstar (
+          CFML.SepBase.SepBasicSetup.HS.repr (Estack re) _prog_re
+        ) (
+          CFML.SepBase.SepBasicSetup.SepSimplArgsCredits.hpure (
+            Coq.Init.Logic.eq (re m) ((pview ps) m)
+          )
+        )
+      )
+    )
+  ).
+
+Parameter _estack_to_pstack : CFML.Semantics.val.
+
+Parameter _estack_to_pstack_spec :
+  forall a : Type,
+  forall {aIh : Inhab a},
+  forall {Ea : CFML.SepLifted.Enc a},
+  forall m : memory a,
+  forall _prog_es : loc,
+  forall es : memory a -> sequence a,
+  CFML.SepLifted.Triple (
+    CFML.SepLifted.Trm_apps _estack_to_pstack (
+      Coq.Lists.List.cons (@CFML.SepLifted.dyn_make (memory a) _ m) (
+        Coq.Lists.List.cons (@CFML.SepLifted.dyn_make loc _ _prog_es) Coq.Lists.List.nil
+      )
+    )
+  ) (CFML.SepBase.SepBasicSetup.HS.repr (Estack es) _prog_es) (
+    fun _res_ : Coq.Init.Datatypes.prod loc (memory a) =>
+    let '(_prog_rp, m') := _res_ in
+    CFML.SepBase.SepBasicSetup.SepSimplArgsCredits.hexists (
+      fun rp : pstack a =>
+      CFML.SepBase.SepBasicSetup.SepSimplArgsCredits.hstar (
+        CFML.SepBase.SepBasicSetup.HS.repr (Pstack rp) _prog_rp
+      ) (
+        CFML.SepBase.SepBasicSetup.SepSimplArgsCredits.hstar (
+          CFML.SepBase.SepBasicSetup.SepSimplArgsCredits.hpure (
+            Coq.Init.Logic.eq ((pview rp) m') (es m)
+          )
+        ) (CFML.SepBase.SepBasicSetup.SepSimplArgsCredits.hpure (extend m m'))
+      )
+    )
+  ).
+
+
