examples/translations/Ref/ref_mli.v
@@ -1,0 +1,91 @@
+Set Implicit Arguments.
+
+Require Import gospelstdlib_verified.
+
+Require Coq.ZArith.BinInt TLC.LibLogic TLC.LibRelation TLC.LibInt TLC.LibListZ.
+
+Require Import CFML.SepBase CFML.SepLifted CFML.WPLib CFML.WPLifted CFML.WPRecord CFML.WPArray CFML.WPBuiltin.
+
+Require CFML.Stdlib.Array_ml CFML.Stdlib.List_ml CFML.Stdlib.Sys_ml.
+
+Require Import Coq.ZArith.BinIntDef CFML.Semantics CFML.WPHeader.
+
+Delimit Scope Z_scope with Z.
+
+Import Stdlib.
+
+Import Gospelstdlib.
+
+Parameter ref : Type -> Type.
+
+Parameter __Enc_ref : forall a : Type, CFML.SepLifted.Enc (ref a).
+
+Instance _Enc_ref : forall a : Type, CFML.SepLifted.Enc (ref a) :=
+__Enc_ref.
+
+Parameter Ref :
+  forall a : Type,
+  forall {aIh : Inhab a},
+  forall {Ea : CFML.SepLifted.Enc a},
+  a -> loc -> CFML.SepBase.SepBasicSetup.SepSimplArgsCredits.hprop.
+
+Parameter _ref : CFML.Semantics.val.
+
+Lemma _ref_spec :
+  forall a : Type,
+  forall {aIh : Inhab a},
+  forall {Ea : CFML.SepLifted.Enc a},
+  forall v : a,
+  CFML.SepLifted.Triple (
+    CFML.SepLifted.Trm_apps _ref (
+      Coq.Lists.List.cons (@CFML.SepLifted.dyn_make a _ v) Coq.Lists.List.nil
+    )
+  ) CFML.SepBase.SepBasicSetup.SepSimplArgsCredits.hempty (
+    fun _prog_r : loc =>
+    CFML.SepBase.SepBasicSetup.HS.repr (Ref v) _prog_r
+  ). Admitted.
+
+Parameter _get : CFML.Semantics.val.
+
+Lemma _get_spec :
+  forall a : Type,
+  forall {aIh : Inhab a},
+  forall {Ea : CFML.SepLifted.Enc a},
+  forall _prog_r : loc,
+  forall r : a,
+  CFML.SepLifted.Triple (
+    CFML.SepLifted.Trm_apps _get (
+      Coq.Lists.List.cons (@CFML.SepLifted.dyn_make loc _ _prog_r) Coq.Lists.List.nil
+    )
+  ) (CFML.SepBase.SepBasicSetup.HS.repr (Ref r) _prog_r) (
+    fun v : a =>
+    CFML.SepBase.SepBasicSetup.SepSimplArgsCredits.hstar (
+      CFML.SepBase.SepBasicSetup.HS.repr (Ref r) _prog_r
+    ) (
+      CFML.SepBase.SepBasicSetup.SepSimplArgsCredits.hpure (
+        Coq.Init.Logic.eq r v
+      )
+    )
+  ). Admitted.
+
+Parameter _update : CFML.Semantics.val.
+
+Lemma _update_spec :
+  forall a : Type,
+  forall {aIh : Inhab a},
+  forall {Ea : CFML.SepLifted.Enc a},
+  forall _prog_r : loc,
+  forall r : a,
+  forall v : a,
+  CFML.SepLifted.Triple (
+    CFML.SepLifted.Trm_apps _update (
+      Coq.Lists.List.cons (@CFML.SepLifted.dyn_make loc _ _prog_r) (
+        Coq.Lists.List.cons (@CFML.SepLifted.dyn_make a _ v) Coq.Lists.List.nil
+      )
+    )
+  ) (CFML.SepBase.SepBasicSetup.HS.repr (Ref r) _prog_r) (
+    fun _ : Coq.Init.Datatypes.unit =>
+    CFML.SepBase.SepBasicSetup.HS.repr (Ref v) _prog_r
+  ). Admitted.
+
+
