examples/translations/Stack_cfml/stack_cfml_mli.v
@@ -1,0 +1,189 @@
+Set Implicit Arguments.
+
+Require Import gospelstdlib_verified.
+
+Require Coq.ZArith.BinInt TLC.LibLogic TLC.LibRelation TLC.LibInt TLC.LibListZ.
+
+Require Import CFML.SepBase CFML.SepLifted CFML.WPLib CFML.WPLifted CFML.WPRecord CFML.WPArray CFML.WPBuiltin.
+
+Require CFML.Stdlib.Array_ml CFML.Stdlib.List_ml CFML.Stdlib.Sys_ml.
+
+Require Import Coq.ZArith.BinIntDef CFML.Semantics CFML.WPHeader.
+
+Delimit Scope Z_scope with Z.
+
+Import Stdlib.
+
+Import Gospelstdlib.
+
+Import Sequence.
+
+Parameter Stack_cfml :
+  forall a : Type,
+  forall {aIh : Inhab a},
+  forall {Ea : CFML.SepLifted.Enc a},
+  sequence a ->
+  loc -> CFML.SepBase.SepBasicSetup.SepSimplArgsCredits.hprop.
+
+Parameter _create : CFML.Semantics.val.
+
+Parameter _create_spec :
+  forall a : Type,
+  forall {aIh : Inhab a},
+  forall {Ea : CFML.SepLifted.Enc a},
+  CFML.SepLifted.Triple (
+    CFML.SepLifted.Trm_apps _create (
+      Coq.Lists.List.cons (
+        @CFML.SepLifted.dyn_make CFML.Semantics.val _ Coq.Init.Datatypes.tt
+      ) Coq.Lists.List.nil
+    )
+  ) CFML.SepBase.SepBasicSetup.SepSimplArgsCredits.hempty (
+    fun _prog_q : loc =>
+    CFML.SepBase.SepBasicSetup.HS.repr (Stack_cfml (@empty a aIh)) _prog_q
+  ).
+
+Parameter _is_empty : CFML.Semantics.val.
+
+Parameter _is_empty_spec :
+  forall a : Type,
+  forall {aIh : Inhab a},
+  forall {Ea : CFML.SepLifted.Enc a},
+  forall _prog_q : loc,
+  forall q : sequence a,
+  CFML.SepLifted.Triple (
+    CFML.SepLifted.Trm_apps _is_empty (
+      Coq.Lists.List.cons (@CFML.SepLifted.dyn_make loc _ _prog_q) Coq.Lists.List.nil
+    )
+  ) (CFML.SepBase.SepBasicSetup.HS.repr (Stack_cfml q) _prog_q) (
+    fun _prog_b : bool =>
+    CFML.SepBase.SepBasicSetup.SepSimplArgsCredits.hstar (
+      CFML.SepBase.SepBasicSetup.HS.repr (Stack_cfml q) _prog_q
+    ) (
+      CFML.SepBase.SepBasicSetup.HS.repr (
+        Bool (Coq.Init.Logic.eq q (@empty a aIh))
+      ) _prog_b
+    )
+  ).
+Parameter _push : CFML.Semantics.val.
+
+Parameter _push_spec :
+  forall a : Type,
+  forall {aIh : Inhab a},
+  forall {Ea : CFML.SepLifted.Enc a},
+  forall _prog_p : loc,
+  forall p : sequence a,
+  forall x : a,
+  CFML.SepLifted.Triple (
+    CFML.SepLifted.Trm_apps _push (
+      Coq.Lists.List.cons (@CFML.SepLifted.dyn_make loc _ _prog_p) (
+        Coq.Lists.List.cons (@CFML.SepLifted.dyn_make a _ x) Coq.Lists.List.nil
+      )
+    )
+  ) (CFML.SepBase.SepBasicSetup.HS.repr (Stack_cfml p) _prog_p) (
+    fun _ : Coq.Init.Datatypes.unit =>
+    CFML.SepBase.SepBasicSetup.HS.repr (Stack_cfml (cons x p)) _prog_p
+  ).
+
+Parameter _pop : CFML.Semantics.val.
+
+Lemma _pop_spec :
+  forall a : Type,
+  forall {aIh : Inhab a},
+  forall {Ea : CFML.SepLifted.Enc a},
+  forall _prog_p : loc,
+  forall p : sequence a,
+  Coq.Init.Logic.not (Coq.Init.Logic.eq p (@empty a aIh)) ->
+  CFML.SepLifted.Triple (
+    CFML.SepLifted.Trm_apps _pop (
+      Coq.Lists.List.cons (@CFML.SepLifted.dyn_make loc _ _prog_p) Coq.Lists.List.nil
+    )
+  ) (CFML.SepBase.SepBasicSetup.HS.repr (Stack_cfml p) _prog_p) (
+    fun r : a =>
+    CFML.SepBase.SepBasicSetup.SepSimplArgsCredits.hexists (
+      fun _p_ : sequence a =>
+      CFML.SepBase.SepBasicSetup.SepSimplArgsCredits.hstar (
+        CFML.SepBase.SepBasicSetup.HS.repr (Stack_cfml _p_) _prog_p
+      ) (
+        CFML.SepBase.SepBasicSetup.SepSimplArgsCredits.hpure (
+          Coq.Init.Logic.eq p (cons r _p_)
+        )
+      )
+    )
+  ). Admitted.
+
+Parameter _clear : CFML.Semantics.val.
+
+Parameter _clear_spec :
+  forall a : Type,
+  forall {aIh : Inhab a},
+  forall {Ea : CFML.SepLifted.Enc a},
+  forall _prog_p : loc,
+  forall p : sequence a,
+  CFML.SepLifted.Triple (
+    CFML.SepLifted.Trm_apps _clear (
+      Coq.Lists.List.cons (@CFML.SepLifted.dyn_make loc _ _prog_p) Coq.Lists.List.nil
+    )
+  ) (CFML.SepBase.SepBasicSetup.HS.repr (Stack_cfml p) _prog_p) (
+    fun _ : Coq.Init.Datatypes.unit =>
+    CFML.SepBase.SepBasicSetup.HS.repr (Stack_cfml (@empty a aIh)) _prog_p
+  ).
+
+Parameter _concat : CFML.Semantics.val.
+
+Parameter _concat_spec :
+  forall a : Type,
+  forall {aIh : Inhab a},
+  forall {Ea : CFML.SepLifted.Enc a},
+  forall _prog_q1 : loc,
+  forall q1 : sequence a,
+  forall _prog_q2 : loc,
+  forall q2 : sequence a,
+  CFML.SepLifted.Triple (
+    CFML.SepLifted.Trm_apps _concat (
+      Coq.Lists.List.cons (@CFML.SepLifted.dyn_make loc _ _prog_q1) (
+        Coq.Lists.List.cons (@CFML.SepLifted.dyn_make loc _ _prog_q2) Coq.Lists.List.nil
+      )
+    )
+  ) (
+    CFML.SepBase.SepBasicSetup.SepSimplArgsCredits.hstar (
+      CFML.SepBase.SepBasicSetup.HS.repr (Stack_cfml q1) _prog_q1
+    ) (CFML.SepBase.SepBasicSetup.HS.repr (Stack_cfml q2) _prog_q2)
+  ) (
+    fun _ : Coq.Init.Datatypes.unit =>
+    CFML.SepBase.SepBasicSetup.SepSimplArgsCredits.hstar (
+      CFML.SepBase.SepBasicSetup.HS.repr (Stack_cfml (app q1 q2)) _prog_q1
+    ) (
+      CFML.SepBase.SepBasicSetup.HS.repr (Stack_cfml (@empty a aIh)) _prog_q2
+    )
+  ).
+
+Parameter _rev_append : CFML.Semantics.val.
+
+Parameter _rev_append_spec :
+  forall a : Type,
+  forall {aIh : Inhab a},
+  forall {Ea : CFML.SepLifted.Enc a},
+  forall _prog_p1 : loc,
+  forall p1 : sequence a,
+  forall _prog_p2 : loc,
+  forall p2 : sequence a,
+  CFML.SepLifted.Triple (
+    CFML.SepLifted.Trm_apps _rev_append (
+      Coq.Lists.List.cons (@CFML.SepLifted.dyn_make loc _ _prog_p1) (
+        Coq.Lists.List.cons (@CFML.SepLifted.dyn_make loc _ _prog_p2) Coq.Lists.List.nil
+      )
+    )
+  ) (
+    CFML.SepBase.SepBasicSetup.SepSimplArgsCredits.hstar (
+      CFML.SepBase.SepBasicSetup.HS.repr (Stack_cfml p1) _prog_p1
+    ) (CFML.SepBase.SepBasicSetup.HS.repr (Stack_cfml p2) _prog_p2)
+  ) (
+    fun _ : Coq.Init.Datatypes.unit =>
+    CFML.SepBase.SepBasicSetup.SepSimplArgsCredits.hstar (
+      CFML.SepBase.SepBasicSetup.HS.repr (Stack_cfml (@empty a aIh)) _prog_p1
+    ) (
+      CFML.SepBase.SepBasicSetup.HS.repr (Stack_cfml (app (rev p1) p2)) _prog_p2
+    )
+  ).
+
+
