examples/translations/Test/test_mli.v
@@ -1,0 +1,57 @@
+Set Implicit Arguments.
+
+Require Import gospelstdlib_verified.
+
+Require Coq.ZArith.BinInt TLC.LibLogic TLC.LibRelation TLC.LibInt TLC.LibListZ.
+
+Require Import CFML.SepBase CFML.SepLifted CFML.WPLib CFML.WPLifted CFML.WPRecord CFML.WPArray CFML.WPBuiltin.
+
+Require CFML.Stdlib.Array_ml CFML.Stdlib.List_ml CFML.Stdlib.Sys_ml.
+
+Require Import Coq.ZArith.BinIntDef CFML.Semantics CFML.WPHeader.
+
+Delimit Scope Z_scope with Z.
+
+Import Stdlib.
+
+Import Gospelstdlib.
+
+Record t : Type := _mk_t { y : int; x : int }.
+
+Parameter _t : Type.
+
+Parameter __Enc__t : CFML.SepLifted.Enc _t.
+
+Instance _Enc__t : CFML.SepLifted.Enc _t := __Enc__t.
+
+Parameter Test :
+  t -> _t -> CFML.SepBase.SepBasicSetup.SepSimplArgsCredits.hprop.
+
+Parameter _f : CFML.Semantics.val.
+
+Parameter _f_spec :
+  forall _prog_arg : _t,
+  forall arg : t,
+  CFML.SepLifted.Triple (
+    CFML.SepLifted.Trm_apps _f (
+      Coq.Lists.List.cons (@CFML.SepLifted.dyn_make _t _ _prog_arg) Coq.Lists.List.nil
+    )
+  ) (CFML.SepBase.SepBasicSetup.HS.repr (Test arg) _prog_arg) (
+    fun _prog_r : _t =>
+    CFML.SepBase.SepBasicSetup.SepSimplArgsCredits.hexists (
+      fun r : t =>
+      CFML.SepBase.SepBasicSetup.SepSimplArgsCredits.hstar (
+        CFML.SepBase.SepBasicSetup.HS.repr (Test arg) _prog_arg
+      ) (
+        CFML.SepBase.SepBasicSetup.SepSimplArgsCredits.hstar (
+          CFML.SepBase.SepBasicSetup.HS.repr (Test r) _prog_r
+        ) (
+          CFML.SepBase.SepBasicSetup.SepSimplArgsCredits.hpure (
+            Coq.Init.Logic.eq (x arg) (y r)
+          )
+        )
+      )
+    )
+  ).
+
+
